add guess example and some changes for autograder

state/Examples.Autograder.fst
@@ -1,15 +1,13 @@
-module Examples
+module Examples.Autograder
 
+open FStar.FiniteSet.Base
+open FStar.Ghost
+open FStar.Monotonic.Heap
 open FStar.Preorder
 open FStar.Tactics.Typeclasses
-open FStar.FiniteSet.Base
+
 open SharedRefs
 open Witnessable
-
-open FStar.Monotonic.Heap (* Remove if we don't use footprint *)
-
-open FStar.Tactics
-open FStar.Ghost
 
 module FSet = FStar.FiniteSet.Base
 
@@ -39,20 +37,6 @@ let rec no_cycles_fuel (fuel:nat) (ll:linkedList int) (h:heap): Type0 =
     match ll with
     | LLNil -> True
     | LLCons x xsref -> no_cycles_fuel (fuel - 1) (sel h xsref) h
-
-let rec no_cycles_ST (fuel: nat) (ll: linkedList int): ST Type0
-  (requires fun h0 -> satisfy_on_heap ll h0 contains_pred)
-  (ensures fun h0 r h1 -> True) =
-  if fuel = 0 then False
-  else
-    match ll with
-      | LLNil -> True
-      | LLCons x xsref -> 
-        let h0 = get_heap() in
-        assert (h0 `contains` xsref);
-        admit(); (* To fix: postcond of read fails *)
-        let tail : linkedList int = sst_read' xsref in
-        no_cycles_ST (fuel - 1) tail
 
 let rec sorted_fuel (fuel:nat) (ll:linkedList int) (h:heap): Type0 =
   if fuel = 0 then False
@@ -95,19 +79,16 @@ let footprint (l: linkedList int) (h:heap) : (GTot (FSet.set nat)) =
   assume (forall (a:Type) (rel:_) (r:mref a rel). h `contains` r ==> addr_of r `FSet.mem` hdom);
   footprint_acc l h hdom FSet.emptyset
 
+let ll_length (ll: linkedList int) (h: heap): GTot int =
+  cardinality (footprint ll h)
+
 let no_cycles (ll:linkedList int) (h:heap): Type0 =
-  let fp = footprint ll h in 
-  let necess_fuel = FSet.cardinality fp + 1 in
+  let necess_fuel = ll_length ll h + 1 in
   no_cycles_fuel necess_fuel ll h
 
 let sorted (ll: linkedList int) (h:heap): Type0 = 
-  let fp = footprint ll h in 
-  let necess_fuel = FSet.cardinality fp + 1 in
+  let necess_fuel = ll_length ll h + 1 in
   sorted_fuel necess_fuel ll h
-
-let element_of_ll' (ll: linkedList int) (h: heap): GTot (Set.set int) = 
-  let fp = set_as_list (footprint ll h) in
-  Set.empty
 
 let rec elements_of_ll_acc (fuel:nat) (ll:linkedList int) (h:heap) (acc: FSet.set int) : GTot (FSet.set int) =
   if fuel = 0 then acc
@@ -123,15 +104,38 @@ let rec elements_of_ll_acc (fuel:nat) (ll:linkedList int) (h:heap) (acc: FSet.se
   elements_of_ll_acc fuel ll h FSet.emptyset *) (* Previously: fuel = max_length *)
 
 let same_elements (ll:linkedList int) (h0 h1:heap): Type0 = 
-  let fp_h0 = footprint ll h0 in
-  let fp_h1 = footprint ll h1 in 
-  let length_fp_h0 = cardinality fp_h0 in
-  let length_fp_h1 = cardinality fp_h1 in
-  if length_fp_h0 <> length_fp_h1 then False
+  let length_h0 = ll_length ll h0 in
+  let length_h1 = ll_length ll h1 in
+  if length_h0 <> length_h1 then False
   else 
-    let fuel_0 = length_fp_h0 + 1 in
-    let fuel_1 = length_fp_h1 + 1 in
-    elements_of_ll_acc fuel_0 ll h0 FSet.emptyset == elements_of_ll_acc fuel_0 ll h0 FSet.emptyset
+    let necess_fuel = length_h0 + 1 in
+    elements_of_ll_acc necess_fuel ll h0 FSet.emptyset == elements_of_ll_acc necess_fuel ll h0 FSet.emptyset
+
+let rec no_cycles_ST (fuel: nat) (ll: linkedList int): SST bool
+  (requires fun h0 -> satisfy_on_heap ll h0 contains_pred)
+  (ensures fun h0 r h1 -> h0 == h1 /\ (r ==> no_cycles ll h1)) =
+  if fuel = 0 then false
+  else
+    match ll with
+      | LLNil -> true
+      | LLCons x xsref -> 
+        let h0 = get_heap() in
+        assert (h0 `contains` xsref);
+        let tail : linkedList int = sst_read' xsref in
+        let h1 = get_heap() in 
+        assert (h0 == h1);
+        admit();
+        no_cycles_ST (fuel - 1) tail
+
+let sorted_ST (ll: linkedList int): SST bool 
+  (requires fun h0 -> satisfy_on_heap ll h0 contains_pred)
+  (ensures fun h0 r h1 -> sorted ll h1) 
+  = admit()
+
+let same_elements_ST (ll: linkedList int): SST bool 
+  (requires fun h0 -> satisfy_on_heap ll h0 contains_pred)
+  (ensures fun h0 r h1 -> same_elements ll h0 == same_elements ll h1) 
+  = admit()
 
 type student_solution =
   ll:linkedList int -> SST (option unit)
@@ -145,10 +149,7 @@ type student_solution =
 let wss : witnessable (list (mref grade grade_preorder * student_solution)) = admit ()
 (*  witnessable_list (witnessable_pair (witnessable_mref witnessable_grade grade_preorder) witnessable_llist) *)
 
-let rec grading_done (sts: list (mref grade grade_preorder * student_solution)) h =
-  match sts with
-  | [] -> True
-  | hd::tl -> sel h (fst hd) =!= NotGraded /\ grading_done tl h
+let rec grading_done (gr: mref grade grade_preorder) h = sel h gr =!= NotGraded
 
 (* TODO: add specs (one postcond should be no cycles) *)
 let rec generate_llist (l:list int)
@@ -160,13 +161,6 @@ let rec generate_llist (l:list int)
   | [] -> LLNil
   | hd::tl -> LLCons hd (sst_alloc_shareable #(SLList SNat) (generate_llist tl))
 
-(* val list_length: fuel:nat -> ll:linkedList int -> Tot nat (decreases fuel) *)
-let rec list_length (fuel: nat) (ll: linkedList int) (h: heap): GTot int =
-  if fuel = 0 then 0
-  else 
-    match ll with
-    | LLNil -> 0
-    | LLCons _ next -> 1 + list_length (fuel - 1) (sel h next) h
 
 let rec share_llist (l:linkedList int) 
   : SST unit 
@@ -174,7 +168,7 @@ let rec share_llist (l:linkedList int)
                          satisfy_on_heap l h0 is_private /\
                          no_cycles l h0))
     (fun h0 r h1 -> satisfy_on_heap r h1 is_shared) 
-    (decreases l) = 
+    (decreases ll_length l) = 
   match l with
   | LLNil -> ()
   | LLCons x next -> 
@@ -193,22 +187,18 @@ let rec share_llist (l:linkedList int)
     share_llist tl
 
 let rec auto_grader
-  (l:list int)
-  (sts: list (mref grade grade_preorder * student_solution))
+  (test:list int)
+  (hw: student_solution) 
+  (gr: mref grade grade_preorder)
   : SST unit
-    (requires (fun h0 -> wss.satisfy_on_heap sts h0 (fun r h0 -> ~(is_shared r h0))))
-    (ensures (fun h0 () h1 ->
-      wss.satisfy_on_heap sts h1 (fun r h0 -> ~(is_shared r h0)) /\
-      grading_done sts h1
-      )) =
-  match sts with
-  | [] -> ()
-  | (gr, hw)::tl -> begin
-    let ll = generate_llist l in
+    (requires (fun h0 -> ~(grading_done gr h0))) (*TODO: add precond from paper *)
+    (ensures (fun h0 () h1 -> grading_done gr h1 /\
+              (forall (a:Type) (rel:FStar.Preorder.preorder a) (r:mref a rel) . 
+                h0 `contains` r ==> kind_not_modified r h0 h1) /\ 
+                modifies !{gr} h0 h1)) =
+    let ll = generate_llist test in
     admit ();
     share_llist ll;
     (match hw ll with
     | Some _ -> sst_write gr MaxGrade
-    | None -> sst_write gr MinGrade);
-    auto_grader l tl
-  end
+    | None -> sst_write gr MinGrade)
