state/Examples.Guess.fst
@@ -1,0 +1,38 @@
+module Examples.Guess
+
+open FStar.FiniteSet.Base
+open FStar.Ghost
+open FStar.Monotonic.Heap
+open FStar.Preorder
+open FStar.Tactics.Typeclasses
+
+open SharedRefs
+open Witnessable
+
+type r = 
+  | LT 
+  | GT 
+  | EQ
+
+(*TODO: check second postcond & update the name here/ in the paper to match *)
+let post_cond = fun h0 _ h1 -> modifies_only_shared_and_encapsulated h0 h1 
+              /\ (forall (a:Type) (rel:FStar.Preorder.preorder a) (r:mref a rel) . 
+                  h0 `contains` r ==> kind_not_modified r h0 h1)
+
+type player_type =
+  l: int -> r: int -> (guess: int -> SST int (requires fun _ -> True) (ensures post_cond)) ->
+  SST int (requires (fun _ -> l < r)) (ensures post_cond)
+
+let play_guess (l pick r: int) (player: player_type) : 
+  SST (bool * int)
+  (requires fun _ -> l < pick /\ pick < r) 
+  (ensures post_cond) =
+  (* let counter = alloc 0 (fun v' v'' -> v' <= v'') in
+  encapsulate counter;
+  let final_guess = 
+    player (fun x -> counter := counter + 1;
+            if pick = x then EQ
+            else if pick < x then GT else LT) in
+  if pick = final_guess then (true, !counter)
+  else (false, !counter) *)
+  admit()
